CpcMini/Lemmas.lean
@@ -14,7 +14,7 @@ set_option maxHeartbeats 10000000
 /- correctness theorem for __eo_prog_scope -/
 theorem correct___eo_prog_scope (M : SmtModel) (x1 x2 : Term) :
   (eo_interprets M x2 true) ->
-  (__eo_prog_scope x1 (Proof.pf x2) ≠ Term.Stuck) ->
+  (Not ((__eo_prog_scope x1 (Proof.pf x2)) = Term.Stuck)) ->
   (eo_interprets M (__eo_prog_scope x1 (Proof.pf x2)) true) :=
 by
   sorry
@@ -23,14 +23,14 @@ by
 theorem correct___eo_prog_contra (M : SmtModel) (x1 x2 : Term) :
   (eo_interprets M x1 true) ->
   (eo_interprets M x2 true) ->
-  (__eo_prog_contra (Proof.pf x1) (Proof.pf x2) ≠ Term.Stuck) ->
+  (Not ((__eo_prog_contra (Proof.pf x1) (Proof.pf x2)) = Term.Stuck)) ->
   (eo_interprets M (__eo_prog_contra (Proof.pf x1) (Proof.pf x2)) true) :=
 by
   sorry
 
 /- correctness theorem for __eo_prog_refl -/
 theorem correct___eo_prog_refl (M : SmtModel) (x1 : Term) :
-  (__eo_prog_refl x1 ≠ Term.Stuck) ->
+  (Not ((__eo_prog_refl x1) = Term.Stuck)) ->
   (eo_interprets M (__eo_prog_refl x1) true) :=
 by
   sorry
@@ -38,7 +38,22 @@ by
 /- correctness theorem for __eo_prog_symm -/
 theorem correct___eo_prog_symm (M : SmtModel) (x1 : Term) :
   (eo_interprets M x1 true) ->
-  (__eo_prog_symm (Proof.pf x1) ≠ Term.Stuck) ->
+  (Not ((__eo_prog_symm (Proof.pf x1)) = Term.Stuck)) ->
   (eo_interprets M (__eo_prog_symm (Proof.pf x1)) true) :=
 by
   sorry
+
+/- correctness theorem for __eo_prog_trans -/
+theorem correct___eo_prog_trans (M : SmtModel) (x1 : Term) :
+  (eo_interprets M x1 true) ->
+  (Not ((__eo_prog_trans (Proof.pf x1)) = Term.Stuck)) ->
+  (eo_interprets M (__eo_prog_trans (Proof.pf x1)) true) :=
+by
+  sorry
+
+
+
+
+/- Helper definitions -/
+
+
